inductive_proof/Ewflag_rid_map.fst
@@ -46,7 +46,14 @@ let do (s:concrete_st) (o:op_t) : concrete_st =
   match o with
   |(_, (rid, Enable)) -> M.upd s rid (fst (sel s rid) + 1, true) 
   |(_, (rid, Disable)) -> M.map_val (fun (c,f) -> (c, false)) s 
-       
+
+type resolve_conflict_res =
+  | First_then_second // op2.op1 
+  | Second_then_first // op1.op2
+
+let resolve_conflict (x:op_t) (y:op_t{fst x <> fst y}) : resolve_conflict_res =
+  if Enable? (snd (snd x)) && Disable? (snd (snd y)) then First_then_second else Second_then_first
+  
 let merge_flag (l a b:cf) : bool =
   let lc = fst l in
   let ac = fst a in
@@ -68,30 +75,99 @@ let concrete_merge (lca s1 s2:concrete_st) : concrete_st =
   M.iter_upd (fun k v -> merge_cf (sel lca k) (sel s1 k) (sel s2 k)) u
 
 #push-options "--z3rlimit 100"
-let prop1 (l:concrete_st) (o1 o2 o3:op_t)
-  : Lemma (requires fst o1 <> fst o3 /\ 
-                    ((Enable? (snd (snd o1)) /\ Enable? (snd (snd o2)) /\ Enable? (snd (snd o3))) \/
-                     (Enable? (snd (snd o1)) /\ Enable? (snd (snd o2)) /\ Disable? (snd (snd o3))) \/
-                     (Enable? (snd (snd o1)) /\ Disable? (snd (snd o2)) /\ Disable? (snd (snd o3))) \/
-                     (Disable? (snd (snd o1)) /\ Enable? (snd (snd o2)) /\ Disable? (snd (snd o3))) \/
-                     (Disable? (snd (snd o1)) /\ Disable? (snd (snd o2)) /\ Disable? (snd (snd o3)))) /\
+let prop1 (l:concrete_st) (o1 o2 o3:op_t) // cond1
+  : Lemma (requires fst o1 <> fst o3 /\ fst o2 <> fst o3 /\ 
+                    resolve_conflict o1 o3 = First_then_second /\
+                    resolve_conflict o2 o3 = First_then_second (*/\
+                    get_rid o1 = get_rid o2 /\ get_rid o3 <> get_rid o1*))
+          (ensures eq (concrete_merge (do l o1) (do (do l o1) o2) (do (do l o3) o1)) (do (do (do l o3) o1) o2)) = ()
+
+let prop2 (s s':concrete_st) (o1 o2 o3:op_t) //cond2
+  : Lemma (requires fst o1 <> fst o3 /\ fst o2 <> fst o3 /\
+                    resolve_conflict o1 o3 = First_then_second /\
+                    resolve_conflict o2 o3 = First_then_second /\
+                    eq (concrete_merge s (do s o2) s') (do s' o2)
+                    (*get_rid o1 = get_rid o2 /\ get_rid o1 <> get_rid o3*))
+          (ensures eq (concrete_merge (do s o1) (do (do s o1) o2) (do s' o1)) (do (do s' o1) o2)) = ()
+
+let prop3 (s s':concrete_st) (o2 o2':op_t)
+  : Lemma (requires eq (concrete_merge s s s') s' /\
+                    ((Enable? (snd (snd o2)) /\ Enable? (snd (snd o2'))) \/
+                     (Enable? (snd (snd o2)) /\ Disable? (snd (snd o2'))) \/
+                     (Disable? (snd (snd o2)) /\ Enable? (snd (snd o2'))) \/
+                     (Disable? (snd (snd o2)) /\ Disable? (snd (snd o2')))) /\
+                    (forall o. eq (concrete_merge s (do s o) s') (do s' o)))
+                    //fst o2 <> fst o2' /\ get_rid o2 = get_rid o2')
+          (ensures eq (concrete_merge s (do (do s o2') o2) s') (do (do s' o2') o2)) = ()
+
+let lem_merge3 (l a b c:concrete_st) (op op':op_t) //cond3
+  : Lemma 
+    (requires eq (concrete_merge l a b) c /\ 
+              ((Enable? (snd (snd op)) /\ Enable? (snd (snd op'))) \/
+               (Enable? (snd (snd op)) /\ Disable? (snd (snd op'))) \/
+               (Disable? (snd (snd op)) /\ Enable? (snd (snd op'))) \/
+               (Disable? (snd (snd op)) /\ Disable? (snd (snd op')))) /\
+              (forall (o:op_t). eq (concrete_merge l a (do b o)) (do c o)))
+              //fst op <> fst op' /\ get_rid op = get_rid op' /\
+    (ensures eq (concrete_merge l a (do (do b op) op')) (do (do c op) op')) = ()
+
+let prop4 (l s:concrete_st) (o1 o2 o3 o3':op_t) //automatic //cond5
+  : Lemma (requires fst o1 <> fst o3 /\ fst o1 <> fst o3' /\ fst o2 <> fst o3 /\ fst o2 <> fst o3' /\
+                    resolve_conflict o1 o3 = First_then_second /\
+                    resolve_conflict o1 o3' = First_then_second /\
+                    resolve_conflict o2 o3 = First_then_second /\
+                    resolve_conflict o2 o3' = First_then_second /\
+                    //get_rid o1 = get_rid o2 /\ get_rid o3 = get_rid o3' /\
+                    //o3.o1, o3'.o1, o3.o2, o3'.o2
+                    eq (concrete_merge (do l o1) (do (do l o1) o2) (do (do s o3) o1)) (do (do (do s o3) o1) o2))
+          (ensures eq (concrete_merge (do l o1) (do (do l o1) o2) (do (do (do s o3') o3) o1)) 
+                      (do (do (do (do s o3') o3) o1) o2)) = ()
+
+let lem_merge4 (s s':concrete_st) (op op':op_t) //cond4
+  : Lemma (requires get_rid op = get_rid op' /\
+                    ((Enable? (snd (snd op)) /\ Enable? (snd (snd op'))) \/
+                    (Enable? (snd (snd op)) /\ Disable? (snd (snd op'))) \/
+                    (Disable? (snd (snd op)) /\ Enable? (snd (snd op'))) \/
+                    (Disable? (snd (snd op)) /\ Disable? (snd (snd op')))) /\
+                    eq (concrete_merge (do s op) (do s' op) (do s op)) (do s' op))
+          (ensures eq (concrete_merge (do s op) (do (do s' op') op) (do s op)) (do (do s' op') op)) = ()
+
+let idempotence (s:concrete_st) //automatic
+  : Lemma (eq (concrete_merge s s s) s) = ()
+
+let prop5' (s:concrete_st) (o:op_t)
+  : Lemma (requires Enable? (snd (snd o)) \/ Disable? (snd (snd o)))
+          (ensures eq (concrete_merge s s (do s o)) (do s o)) = ()
+
+let merge_pre l a b =
+  (forall id. M.contains (concrete_merge l a b) id ==>
+         fst (sel a id) >= fst (sel l id) /\
+         fst (sel b id) >= fst (sel l id))
+               
+let prop5 (s s':concrete_st) (o:op_t)
+  : Lemma (requires eq (concrete_merge s s s') s' /\
+                    merge_pre s s s' /\
+                    (Enable? (snd (snd o)) \/ Disable? (snd (snd o))))
+          (ensures eq (concrete_merge s s (do s' o)) (do s' o)) = ()
+#pop-options
+
+(*#push-options "--z3rlimit 100"
+let prop1 (l:concrete_st) (o1 o2 o3:op_t) // cond1
+  : Lemma (requires fst o1 <> fst o3 /\ fst o2 <> fst o3 /\ 
+                    not (resolve_conflict o3 o1 = First_then_second) /\
+                    not (resolve_conflict o3 o2 = First_then_second) /\
                     get_rid o1 = get_rid o2 (*/\ get_rid o3 <> get_rid o1*))
                     //resolve_conflict o1 o3 = First_then_second) //o3.o1
                     //not (resolve_conflict o2 o3 = Second_then_first) //not(o2.o3)
           (ensures eq (concrete_merge (do l o1) (do (do l o1) o2) (do (do l o3) o1)) (do (do (do l o3) o1) o2)) = ()
 
-let prop2 (l s s':concrete_st) (o1 o2 o3:op_t) 
+let prop2 (l s s':concrete_st) (o1 o2 o3:op_t) //cond2
   : Lemma (requires eq (concrete_merge s (do s o2) s') (do s' o2) /\
-                    ((Enable? (snd (snd o1)) /\ Enable? (snd (snd o2)) /\ Enable? (snd (snd o3))) \/
-                     (Enable? (snd (snd o1)) /\ Enable? (snd (snd o2)) /\ Disable? (snd (snd o3))) \/
-                     (Enable? (snd (snd o1)) /\ Disable? (snd (snd o2)) /\ Enable? (snd (snd o3))) \/
-                     (Enable? (snd (snd o1)) /\ Disable? (snd (snd o2)) /\ Disable? (snd (snd o3))) \/
-                     (Disable? (snd (snd o1)) /\ Enable? (snd (snd o2)) /\ Enable? (snd (snd o3))) \/
-                     (Disable? (snd (snd o1)) /\ Enable? (snd (snd o2)) /\ Disable? (snd (snd o3))) \/
-                     (Disable? (snd (snd o1)) /\ Disable? (snd (snd o2)) /\ Enable? (snd (snd o3))) \/
-                     (Disable? (snd (snd o1)) /\ Disable? (snd (snd o2)) /\ Disable? (snd (snd o3)))) /\
-                    eq (concrete_merge l s (do l o3)) s' (*/\
-                    get_rid o1 = get_rid o2 /\ get_rid o1 <> get_rid o3*))
+                    fst o1 <> fst o3 /\ fst o2 <> fst o3 /\
+                    //not (resolve_conflict o3 o1 = First_then_second) /\
+                    not (resolve_conflict o3 o2 = First_then_second) /\
+                    eq (concrete_merge l s (do l o3)) s' //extra
+                    (*get_rid o1 = get_rid o2 /\ get_rid o1 <> get_rid o3*))
           (ensures eq (concrete_merge (do s o1) (do (do s o1) o2) (do s' o1)) (do (do s' o1) o2)) = ()
 
 let prop3 (s s':concrete_st) (o2 o2':op_t)
@@ -104,7 +180,7 @@ let prop3 (s s':concrete_st) (o2 o2':op_t)
                     fst o2 <> fst o2' /\ get_rid o2 = get_rid o2')
           (ensures eq (concrete_merge s (do (do s o2') o2) s') (do (do s' o2') o2)) = ()
 
-let lem_merge3 (l a b c:concrete_st) (op op':op_t) 
+let lem_merge3 (l a b c:concrete_st) (op op':op_t) //cond3
   : Lemma 
     (requires eq (concrete_merge l a b) c /\ 
               ((Enable? (snd (snd op)) /\ Enable? (snd (snd op'))) \/
@@ -115,23 +191,20 @@ let lem_merge3 (l a b c:concrete_st) (op op':op_t)
               (forall (o:op_t). eq (concrete_merge l a (do b o)) (do c o)))
     (ensures eq (concrete_merge l a (do (do b op) op')) (do (do c op) op')) = ()
 
-let prop4 (l s:concrete_st) (o1 o2 o3 o3':op_t) //automatic
-  : Lemma (requires //fst o2 <> fst o3 /\ 
-                    ((Enable? (snd (snd o1)) /\ Enable? (snd (snd o3))) \/
-                     (Disable? (snd (snd o3)))) /\
-                    ((Enable? (snd (snd o2)) /\ Enable? (snd (snd o3))) \/
-                     (Disable? (snd (snd o3)))) /\
-                    ((Enable? (snd (snd o1)) /\ Enable? (snd (snd o3'))) \/
-                     (Disable? (snd (snd o3')))) /\
-                    ((Enable? (snd (snd o2)) /\ Enable? (snd (snd o3'))) \/
-                     (Disable? (snd (snd o3')))) /\
+let prop4 (l s:concrete_st) (o1 o2 o3 o3':op_t) //automatic //cond5
+  : Lemma (requires fst o1 <> fst o3 /\ fst o1 <> fst o3' /\ fst o2 <> fst o3 /\ fst o2 <> fst o3' /\
+                    //not (resolve_conflict o3 o1 = First_then_second) /\
+                    //not (resolve_conflict o3' o1 = First_then_second) /\
+                    //not (resolve_conflict o3 o2 = First_then_second) /\
+                    not (resolve_conflict o3' o2 = First_then_second) /\
+                    eq (concrete_merge l (do (do l o1) o2) s) (do (do s o1) o2) /\
                     (*get_rid o1 = get_rid o2 /\*) get_rid o3 = get_rid o3' /\
                     //o3.o1, o3'.o1, o3.o2, o3'.o2
                     eq (concrete_merge (do l o1) (do (do l o1) o2) (do (do s o3) o1)) (do (do (do s o3) o1) o2))
           (ensures eq (concrete_merge (do l o1) (do (do l o1) o2) (do (do (do s o3') o3) o1)) 
                       (do (do (do (do s o3') o3) o1) o2)) = ()
 
-let lem_merge4 (s s':concrete_st) (op op':op_t)
+let lem_merge4 (s s':concrete_st) (op op':op_t) //cond4
   : Lemma (requires get_rid op = get_rid op' /\
                     ((Enable? (snd (snd op)) /\ Enable? (snd (snd op'))) \/
                     (Enable? (snd (snd op)) /\ Disable? (snd (snd op'))) \/
@@ -145,16 +218,11 @@ let idempotence (s:concrete_st) //automatic
 
 let prop5' (l s s':concrete_st) (o o3:op_t)
   : Lemma (requires eq (concrete_merge s s s') s' /\
-                    eq (concrete_merge l s (do l o3)) s' /\
+                    eq (concrete_merge l s (do l o3)) s' /\ //extra
                     ((Enable? (snd (snd o)) /\ Enable? (snd (snd o3))) \/
                     (Enable? (snd (snd o)) /\ Disable? (snd (snd o3))) \/
                     (Disable? (snd (snd o)) /\ Enable? (snd (snd o3))) \/
                     (Disable? (snd (snd o)) /\ Disable? (snd (snd o3)))) /\
                     get_rid o <> get_rid o3)
           (ensures eq (concrete_merge s s (do s' o)) (do s' o)) = ()
-
-let prop5 (s s':concrete_st)
-  : Lemma (ensures (//eq_id (concrete_merge s s s') s' /\ 
-                    eq (concrete_merge s s' s) s')) = 
-  admit()
-#pop-options
+#pop-options*)
